src/Rupicola/Examples/ECC/Exponentiation.v
@@ -10,9 +10,6 @@ Section S.
           {semantics_ok : Semantics.parameters_ok semantics}.
   Context {field_parameters : FieldParameters}.
   Context {bignum_representaton : BignumRepresentation}.
-  Existing Instances spec_of_mul spec_of_square spec_of_add
-           spec_of_sub spec_of_scmula24 spec_of_inv spec_of_bignum_copy
-           spec_of_bignum_literal.
 
   Context {relax_bounds :
              forall X : bignum,
